Validator/Expr/Compress.lean
@@ -1,60 +1,397 @@
+import Validator.Std.Vec
+
 import Validator.Expr.Regex
 import Validator.Expr.Grammar
 
 namespace Compress
 
-inductive Index where
- | val (n: Nat)
+inductive Index n where
+ | val (i: Fin n)
  | emptyset -- emptyset is unescapable, so it gets a special index
-
-def indexOf [DecidableEq α] (xs: Rules μ α Pred) (y: (Rule μ α Pred)): Except String Index :=
-  match y with
-  | Regex.emptyset => Except.ok Index.emptyset
-  | _ =>
-    match List.idxOf? y xs with
-    | Option.none => Except.error "indexOf: unable to find expression"
-    | Option.some idx => Except.ok (Index.val idx)
-
-def ofIndex' (xs: Rules μ α Pred) (index: Nat): Except String (Rule μ α Pred) :=
-  match xs with
-  | [] => Except.error "index overflow"
-  | (x::xs') =>
-    match index with
-    | 0 => Except.ok x
-    | (n' + 1) => ofIndex' xs' n'
-
-def ofIndex (xs: Rules μ α Pred) (index: Index): Except String (Rule μ α Pred) :=
-  match index with
-  | Index.emptyset => Except.ok Regex.emptyset
-  | Index.val n =>
-    ofIndex' xs n
 
 -- Indices represents compressed indexes
 -- that resulted from compressing a list of expressions.
 -- This can be used to expanded to a list of expressions.
-inductive Indices where
-  | mk (indices: List Index)
+abbrev Indices (compressed: Nat) (expanded: Nat) :=
+  List.Vector (Index compressed) expanded
 
--- compress compresses a list of expressions.
-def compress [DecidableEq α] (xs: Rules μ α Pred): Except String ((Rules μ α Pred) × Indices) := do
+def eraseReps' [DecidableEq α] (x: α) (xs: List α): List α :=
+  match xs with
+  | [] => [x]
+  | (x'::xs) =>
+    if x == x'
+    then eraseReps' x' xs
+    else x :: eraseReps' x' xs
+
+def eraseReps [DecidableEq α] (xs: List α): List α :=
+  match xs with
+  | [] => []
+  | (x::xs) => eraseReps' x xs
+
+theorem eraseReps_member [DecidableEq α] {xs: List α}:
+  (x ∈ xs) -> (x ∈ eraseReps xs) := by
+  unfold eraseReps
+  intro hxs
+  cases xs with
+  | nil =>
+    simp at hxs
+  | cons x' xs =>
+    simp
+    fun_induction eraseReps'
+    case case1 x' =>
+      assumption
+    case case2 x' x'' xs hc ih =>
+      simp at hc
+      subst hc
+      apply ih
+      simp_all only [List.mem_cons, or_self_left]
+    case case3 x' x'' xs hc ih =>
+      simp at hc
+      simp at hxs
+      simp
+      -- aesop?
+      simp_all only [List.mem_cons]
+      cases hxs with
+      | inl h =>
+        subst h
+        simp_all only [false_or, true_or]
+      | inr h_1 =>
+        cases h_1 with
+        | inl h =>
+          subst h
+          simp_all only [true_or, forall_const, or_true]
+        | inr h_2 => simp_all only [or_true, forall_const]
+
+def eraseReps_sub [DecidableEq α] (xs: List α): { ys: List α // ∀ x ∈ xs, x ∈ ys } :=
+  let ys := eraseReps xs
+  Subtype.mk ys (by
+    subst ys
+    intro x
+    intro hxs
+    apply eraseReps_member hxs
+  )
+
+def idxOf? [DecidableEq α] (xs : List α) (y: α) (i : Nat := 0) : Option Nat :=
+  match xs with
+  | [] => Option.none
+  | (x::xs) =>
+    if x == y
+    then Option.some i
+    else idxOf? xs y (i + 1)
+
+theorem idxOf_length' [DecidableEq α] {y: α} (h: idxOf? xs y n = some i):
+  i < List.length xs + n := by
+  induction xs generalizing i n with
+  | nil =>
+    simp [idxOf?] at h
+  | cons x xs ih =>
+    simp [idxOf?] at h
+    split_ifs at h
+    case pos hxy =>
+      simp_all
+    case neg hxy =>
+      simp_all
+      have ih' := @ih (n + 1)
+      rw [Nat.add_assoc]
+      nth_rewrite 2 [Nat.add_comm]
+      apply ih' h
+
+theorem idxOf_length [DecidableEq α] {y: α} (h: idxOf? xs y = some i):
+  i < List.length xs := by
+  apply idxOf_length' (n := 0) h
+
+theorem idxOf?_eq_none_iff' [DecidableEq α] {xs : List α} {y : α} :
+  idxOf? xs y i = none ↔ y ∉ xs := by
+  induction xs generalizing i with
+  | nil =>
+    simp [idxOf?]
+  | cons x xs ih =>
+    simp [idxOf?]
+    split_ifs
+    case pos h =>
+      subst_vars
+      -- aesop?
+      simp_all only [not_true_eq_false, false_and]
+    case neg h =>
+      have ih' := ih (i := i + 1)
+      -- aesop?
+      simp_all only [iff_and_self]
+      intro a
+      simp_all only [not_false_eq_true, iff_true]
+      apply Aesop.BuiltinRules.not_intro
+      intro a_1
+      subst a_1
+      simp_all only [not_true_eq_false]
+
+theorem idxOf?_eq_none_iff [DecidableEq α] {xs : List α} {y : α} :
+  idxOf? xs y = none ↔ y ∉ xs := by
+  apply idxOf?_eq_none_iff' (i := 0)
+
+def indices [DecidableEq α] {xs: List α} (ys: { ys': List α // ∀ x ∈ xs, x ∈ ys' }): List.Vector (Fin (List.length ys.val)) (List.length xs) :=
+  match xs with
+  | [] => List.Vector.nil
+  | (x::xs) =>
+    match hi: idxOf? ys.val x with
+    | Option.none => by
+      cases ys with
+      | mk ys hys =>
+      simp only [List.mem_cons, forall_eq_or_imp] at hys
+      obtain ⟨left, right⟩ := hys
+      simp only at hi
+      simp_all only [idxOf?_eq_none_iff, List.mem_cons, true_or, not_true_eq_false]
+    | Option.some i =>
+      List.Vector.cons
+        (
+          Fin.mk
+            i
+            (by
+              cases ys with
+              | mk ys hys =>
+              simp only
+              simp only [List.mem_cons, forall_eq_or_imp] at hys
+              obtain ⟨left, right⟩ := hys
+              simp only at hi
+              apply idxOf_length hi
+            )
+        )
+        (indices (xs := xs)
+          (Subtype.mk
+            ys.val
+            (by
+              intro x'
+              intro hxs
+              cases ys with
+              | mk ys hys =>
+              simp only
+              simp only at hi
+              simp_all only [List.mem_cons, forall_eq_or_imp]
+            )
+          )
+        )
+
+def vector_cast (h: n = m) (xs: List.Vector α n): List.Vector α m := by
+  subst h
+  exact xs
+
+def compress [DecidableEq α] (xs: Rules n (Pred α) l1): Σ l2, ((Rules n (Pred α) l2) × (Indices l2 l1)) :=
+  let xs_list: List (Rule n (Pred α)) := xs.toList
+  have hn : xs_list.length = l1 := by
+    simp_all only [List.Vector.toList_length, xs_list]
+
   -- sort to increase chance of cache hit
   -- TODO: let sxs := List.mergeSort xs
-  -- remove duplicates
-  let sxs' := List.eraseReps xs
-  -- remove unescapable expressions, currently only emptyset
-  let sxs'': Rules μ α Pred := List.erase sxs' Regex.emptyset
-  -- find all indexes of the original expressions in the compressed expressions
-  let indexes: List Index <- List.mapM (indexOf sxs'') xs
-  return (sxs'', Indices.mk indexes)
 
-def compressM [DecidableEq α] [Monad m] [MonadExcept String m] (xs: Rules μ α Pred): m ((Rules μ α Pred) × Indices) := do
-  MonadExcept.ofExcept (compress xs)
+  -- remove duplicates
+  let xs_noreps: { ys: List (Rule n (Pred α)) // ∀ x ∈ xs_list, x ∈ ys } := eraseReps_sub xs_list
+
+  -- get indices
+  let xs_idxs: List.Vector (Fin (xs_noreps.val).length) (List.length xs_list) := indices xs_noreps
+
+  -- remove unescapable expressions, currently only emptyset
+  -- TODO: let xs_compressed_list := erase xs_noreps Regex.emptyset
+
+  -- find all indexes of the original expressions in the compressed expressions
+  let indices: Indices (xs_noreps.val).length (List.length xs_list) := List.Vector.map (fun x => Index.val x) xs_idxs
+  let indices': Indices (xs_noreps.val).length l1 := vector_cast hn indices
+
+  Sigma.mk (List.length (xs_noreps.val)) (
+    Subtype.mk xs_noreps rfl,
+    indices'
+  )
+
+def memVector (xs: List.Vector α l) (y: α): Prop :=
+  match xs with
+  | ⟨[], _⟩ => False
+  | ⟨x::xs, h⟩ => x = y \/ memVector ⟨xs, congrArg Nat.pred h⟩ y
+
+instance [DecidableEq α]: Membership α (List.Vector α l) where
+  mem := memVector
+
+theorem memVector_nil {n: Nat} {hxs: [].length = n}
+  (h : memVector (Subtype.mk [] hxs) y): False := by
+  unfold memVector at h
+  exact h
+
+theorem length_cons
+  (h: (x::xs).length = n): xs.length = n - 1 := by
+  simp at h
+  omega
+
+theorem memVector_cons {n: Nat} {hxs: (x::xs).length = n}
+  (h : memVector (Subtype.mk (x::xs) hxs) y)
+  (hnxy : x ≠ y): memVector (Subtype.mk xs (length_cons hxs)) y := by
+  simp [memVector] at h
+  cases h with
+  | inl h =>
+    subst_vars
+    contradiction
+  | inr h =>
+    generalize_proofs at h
+    exact h
+
+def indexOf' [DecidableEq α] (xs: List.Vector α l) (y: α) (h: y ∈ xs): Fin (xs.length) :=
+  match xs with
+  | ⟨[], hxs⟩ => by
+    exfalso
+    apply memVector_nil h
+  | ⟨x::xs, hxs⟩ =>
+    if hxy: x == y
+    then
+      Fin.mk 0 (by
+        simp [List.Vector.length]
+        subst hxs
+        simp [List.length]
+      )
+    else
+      let i := indexOf' ⟨xs, congrArg Nat.pred hxs⟩ y (by
+        simp only [beq_iff_eq] at hxy
+        exact memVector_cons (hxs := hxs) h hxy
+      )
+      Fin.mk (i.val + 1) (by
+        simp [List.Vector.length]
+        subst_vars
+        omega
+      )
+
+theorem memVector_emptyset [DecidableEq α] {y: Regex α}
+  (h1 : memVector (Subtype.mk xs hxs) y ∨ y = Regex.emptyset)
+  (h2 : ¬y == Regex.emptyset): memVector (Subtype.mk xs hxs) y := by
+  cases h1 with
+  | inl h =>
+    exact h
+  | inr h =>
+    simp only [beq_iff_eq] at h2
+    contradiction
+
+def indexOf [DecidableEq α] (xs: List.Vector (Regex α) l) (y: Regex α) (h: y ∈ xs \/ y = Regex.emptyset): Index (xs.length) :=
+  if hy: y == Regex.emptyset
+  then Index.emptyset
+  else Index.val (indexOf' xs y (memVector_emptyset h hy))
+
+def ofIndex' (xs: Rules n (Pred α) l) (index: Fin l): Rule n (Pred α) :=
+  xs.get index
+
+def ofIndex (xs: Rules n (Pred α) l) (index: Index l): Rule n (Pred α) :=
+  match index with
+  | Index.emptyset => Regex.emptyset
+  | Index.val n => ofIndex' xs n
+
+def compressed [DecidableEq σ] (xs: List.Vector (Regex σ) l): Nat :=
+  (List.erase (List.eraseReps xs.toList) Regex.emptyset).length
+
+def numReps [DecidableEq α] (xs: List.Vector α l) (x: Option α := Option.none): Nat :=
+  match x with
+  | Option.none =>
+    match xs with
+    | ⟨[], _⟩ => 0
+    | ⟨x::xs, h⟩ => numReps ⟨xs, congrArg Nat.pred h⟩ (Option.some x)
+  | Option.some x =>
+    match xs with
+    | ⟨[], _⟩ => 0
+    | ⟨x'::xs, h⟩ =>
+      if x == x'
+      then 1 + numReps ⟨xs, congrArg Nat.pred h⟩ (Option.some x')
+      else numReps ⟨xs, congrArg Nat.pred h⟩ (Option.some x')
+
+theorem numReps_none_le_length [DecidableEq α] (xs: List.Vector α l):
+  numReps xs Option.none <= xs.length := by
+  induction xs with
+  | nil =>
+    simp only [List.Vector.nil, numReps, le_refl]
+  | cons ih =>
+    rename_i n x xs
+    simp [List.Vector.cons]
+    split
+    simp [numReps]
+    unfold numReps
+    split
+    · omega
+    · split_ifs
+      case pos h =>
+        simp [List.Vector.length]
+        rename_i h_2 heq
+        subst h_2
+        simp_all only [List.length_cons, Subtype.mk.injEq, Nat.add_one_sub_one]
+        subst heq
+        simp_all only [List.length_cons]
+        simp [numReps] at ih
+        simp [List.Vector.length] at ih
+        omega
+      case neg h =>
+        rename_i h_2 heq
+        subst h_2
+        simp_all only [Bool.not_eq_true, List.length_cons, Subtype.mk.injEq, Nat.pred_eq_sub_one, Nat.add_one_sub_one]
+        subst heq
+        simp_all only [List.length_cons]
+        simp [numReps] at ih
+        simp [List.Vector.length]
+        simp [List.Vector.length] at ih
+        omega
+
+theorem numReps_some_le_length [DecidableEq α] (xs: List.Vector α l):
+  numReps xs (Option.some y) <= xs.length := by
+  induction xs generalizing y with
+  | nil =>
+    simp only [List.Vector.nil, List.Vector.length]
+    unfold numReps
+    split
+    · omega
+    · contradiction
+  | cons ih =>
+    rename_i n x xs
+    simp only [Nat.succ_eq_add_one, List.Vector.cons]
+    split
+    simp only [List.Vector.length] at *
+    rename_i xs xs' hxs'
+    simp [numReps]
+    split_ifs
+    case pos h =>
+      simp only at h
+      subst_vars
+      have ih' := ih (y := y)
+      omega
+    case neg h =>
+      generalize_proofs
+      have ih' := ih (y := x)
+      omega
+
+theorem numReps_le_length [DecidableEq α] (xs: List.Vector α l) (y: Option α):
+  numReps xs y <= xs.length := by
+  cases y with
+  | none =>
+    apply numReps_none_le_length
+  | some y =>
+    apply numReps_some_le_length
+
+def smallest [DecidableEq α] [LT α] [DecidableLT α] (xs: List.Vector α l) (y: α): Option (Fin l) :=
+  match xs with
+  | ⟨[], h⟩ => Option.none
+  | ⟨x::xs, h⟩ =>
+    if x < y
+    then
+      match smallest ⟨xs, congrArg Nat.pred h⟩ x with
+      | Option.none => Option.some ⟨0, by
+          subst h
+          simp
+        ⟩
+      | Option.some n => Option.some ⟨n + 1, by
+          subst h
+          simp
+        ⟩
+    else
+      match smallest ⟨xs, congrArg Nat.pred h⟩ y with
+      | Option.none => Option.none
+      | Option.some n => Option.some ⟨n + 1, by
+          subst h
+          simp
+        ⟩
+
+def compressM [DecidableEq α] [Monad m] (xs: Rules n (Pred α) l1): m (Σ l2, (Rules n (Pred α) l2) × Indices l2 l1) := do
+  return compress xs
 
 -- expand expands a list of expressions.
-def expand (indices: Indices) (xs: Rules μ α Pred): Except String (Rules μ α Pred) :=
-  match indices with
-  | Indices.mk indexes =>
-    List.mapM (ofIndex xs) indexes
+def expand (indices: Indices l1 l2) (xs: Rules n (Pred α) l1): (Rules n (Pred α) l2) :=
+  List.Vector.map (ofIndex xs) indices
 
-def expandM [Monad m] [MonadExcept String m] (indices: Indices) (xs: Rules μ α Pred): m (Rules μ α Pred) :=
-  MonadExcept.ofExcept (expand indices xs)
+def expandM [Monad m] (indices: Indices l1 l2) (xs: Rules n (Pred α) l1): m (Rules n (Pred α) l2) :=
+  return (expand indices xs)
