Validator/Expr/IfExpr.lean
@@ -1,30 +1,27 @@
+import Validator.Std.Vec
+
 import Validator.Expr.Pred
 import Validator.Expr.Regex
 import Validator.Expr.Grammar
 
-inductive IfExpr μ α where
-  | mk (cnd: Pred α) (thn: Fin μ)
+inductive IfExpr n α where
+  | mk (cnd: Pred α) (thn: Fin n)
 
-abbrev IfExprs μ α := List (IfExpr μ α)
+abbrev IfExprs n α l := List.Vector (IfExpr n α) l
 
 namespace IfExpr
 
-def eval {α: Type} [DecidableEq α] (g: Grammar μ α Pred) (ifExpr: IfExpr μ α) (t: α): Rule μ α Pred :=
+def eval {α: Type} [DecidableEq α] (g: Grammar n (Pred α)) (ifExpr: IfExpr n α) (t: α): Rule n (Pred α) :=
   match ifExpr with
   | IfExpr.mk cnd thn =>
     if Pred.eval cnd t
     then g.lookup thn
     else Regex.emptyset
 
-def evals {α: Type} {μ: Nat} [DecidableEq α] (g: Grammar μ α Pred) (ifExprs: IfExprs μ α) (t: α): List (Rule μ α Pred) :=
-  List.map (fun x => eval g x t) ifExprs
+def evals {α: Type} {n: Nat} [DecidableEq α] (g: Grammar n (Pred α)) (ifExprs: IfExprs n α l) (t: α): Rules n (Pred α) l :=
+  List.Vector.map (fun x => eval g x t) ifExprs
 
-theorem evals_nil_is_nil {α: Type} {μ: Nat} [DecidableEq α] (g: Grammar μ α Pred) (a: α):
-  evals g (μ := μ) [] a = [] := by
-  unfold evals
-  simp
-
-theorem evals_concat_is_concat {α: Type} [DecidableEq α] (g: Grammar μ α Pred) (xs ys: IfExprs μ α) (a: α):
-  evals g (xs ++ ys) a = evals g xs a ++ evals g ys a := by
+theorem evals_nil_is_nil {α: Type} {n: Nat} [DecidableEq α] (g: Grammar n (Pred α)) (a: α):
+  evals g (n := n) List.Vector.nil a = List.Vector.nil := by
   unfold evals
   simp
