Validator/Expr/Symbol.lean
@@ -1,5 +1,5 @@
-import Mathlib.Data.Vector.Basic
-import Mathlib.Data.Vector.Snoc
+import Validator.Std.Vec
+
 import Validator.Expr.Regex
 
 -- I want to define a map function over a regular expression:
@@ -41,66 +41,64 @@ def num (r: Regex σ): Nat :=
   | Regex.concat r1 r2 => num r1 + num r2
   | Regex.star r1 => num r1
 
+def nums (xs: List.Vector (Regex σ) l): Nat :=
+  match xs with
+  | ⟨[], _⟩ => 0
+  | ⟨x::xs, h⟩ => nums ⟨xs, congrArg Nat.pred h⟩ + num x
+
+def nums_list (xs: List (Regex σ)): Nat :=
+  nums (Vec.fromList xs)
+
 abbrev RegexID n := Regex (Fin n)
-abbrev Symbols σ n := List.Vector σ n
+abbrev Symbols σ l := List.Vector σ l
 
 def RegexID.add {n: Nat} (m: Nat) (r: RegexID n): RegexID (n + m) :=
   Regex.map r (fun s => (Fin.mk s.val (by omega)))
 
-def RegexID.cast (h: n = m) (r: RegexID n): RegexID m := by
+def RegexID.cast (r: RegexID n) (h: n = m): RegexID m := by
   rw [<- h]
   exact r
 
-def RegexID.add_or (r: RegexID (μ + num r1 + num r2)): RegexID (μ + num (Regex.or r1 r2)) :=
-  have h : (μ + num r1 + num r2) = (μ + num (Regex.or r1 r2)) := by
+def RegexID.add_or (r: RegexID (n + num r1 + num r2)): RegexID (n + num (Regex.or r1 r2)) :=
+  have h : (n + num r1 + num r2) = (n + num (Regex.or r1 r2)) := by
     rw [<- Nat.add_assoc]
-  RegexID.cast h r
+  RegexID.cast r h
 
-def RegexID.add_concat (r: RegexID (μ + num r1 + num r2)): RegexID (μ + num (Regex.concat r1 r2)) :=
-  have h : (μ + num r1 + num r2) = (μ + num (Regex.concat r1 r2)) := by
+def RegexID.add_concat (r: RegexID (n + num r1 + num r2)): RegexID (n + num (Regex.concat r1 r2)) :=
+  have h : (n + num r1 + num r2) = (n + num (Regex.concat r1 r2)) := by
     rw [<- Nat.add_assoc]
-  RegexID.cast h r
+  RegexID.cast r h
 
-theorem List.Vector.toList_take:
-  List.take n xs.val = (List.Vector.take n xs).toList := by
-  simp only [_root_.List.Vector.toList_take]
-  rfl
-
-theorem List.Vector.toList_cons:
-  List.cons x xs.val = (List.Vector.cons x xs).toList := by
-  simp only [Nat.succ_eq_add_one, _root_.List.Vector.toList_cons, List.cons.injEq, true_and]
-  rfl
-
-def Symbols.cast (h: n = m) (xs: Symbols σ n): Symbols σ m := by
+def Symbols.cast (xs: Symbols σ n) (h: n = m): Symbols σ m := by
   rw [<- h]
   exact xs
 
 theorem List.Vector.toList_cast_is_toList (xs: List.Vector σ n):
-  List.Vector.toList xs = List.Vector.toList (Symbols.cast h xs) := by
+  List.Vector.toList xs = List.Vector.toList (Symbols.cast xs h) := by
   rcases xs with ⟨xs, hxs⟩
   simp [Symbols.cast, _root_.cast, List.Vector.toList]
   subst h hxs
   simp only
 
-abbrev Symbols.take {α: Type} (i: Nat) (xs: List.Vector α n) := List.Vector.take i xs
-abbrev Symbols.get {α: Type} (xs: List.Vector α n) (i: Fin n) := List.Vector.get xs i
+abbrev Symbols.take {α: Type} (i: Nat) (xs: List.Vector α l) := List.Vector.take i xs
+abbrev Symbols.get {α: Type} (xs: List.Vector α l) (i: Fin l) := List.Vector.get xs i
 abbrev Symbols.nil {α: Type} := @List.Vector.nil α
-abbrev Symbols.snoc {α: Type} (xs: List.Vector α n) (x: α) := List.Vector.snoc xs x
-abbrev Symbols.cons {α: Type} (x: α) (xs: List.Vector α n) := List.Vector.cons x xs
-abbrev Symbols.set {α: Type} (v : List.Vector α n) (i : Fin n) (a : α) := List.Vector.set v i a
-abbrev Symbols.toList {α: Type} (v : List.Vector α n) := List.Vector.toList v
+abbrev Symbols.snoc {α: Type} (xs: List.Vector α l) (x: α) := List.Vector.snoc xs x
+abbrev Symbols.cons {α: Type} (x: α) (xs: List.Vector α l) := List.Vector.cons x xs
+abbrev Symbols.set {α: Type} (v : List.Vector α l) (i : Fin l) (a : α) := List.Vector.set v i a
+abbrev Symbols.toList {α: Type} (v : List.Vector α l) := List.Vector.toList v
 
-def Symbols.add_or (xs: Symbols σ (μ + num r1 + num r2)): Symbols σ (μ + num (Regex.or r1 r2)) :=
-  have h : (μ + num r1 + num r2) = (μ + num (Regex.or r1 r2)) := by
+def Symbols.add_or (xs: Symbols σ (n + num r1 + num r2)): Symbols σ (n + num (Regex.or r1 r2)) :=
+  have h : (n + num r1 + num r2) = (n + num (Regex.or r1 r2)) := by
     rw [<- Nat.add_assoc]
-  Symbols.cast h xs
+  Symbols.cast xs h
 
-def Symbols.add_concat (xs: Symbols σ (μ + num r1 + num r2)): Symbols σ (μ + num (Regex.or r1 r2)) :=
-  have h : (μ + num r1 + num r2) = (μ + num (Regex.concat r1 r2)) := by
+def Symbols.add_concat (xs: Symbols σ (n + num r1 + num r2)): Symbols σ (n + num (Regex.or r1 r2)) :=
+  have h : (n + num r1 + num r2) = (n + num (Regex.concat r1 r2)) := by
     rw [<- Nat.add_assoc]
-  Symbols.cast h xs
+  Symbols.cast xs h
 
-theorem Symbols.cast_rfl {xs : Symbols α n} : Symbols.cast rfl xs = xs := by
+theorem Symbols.cast_rfl {xs : Symbols α n} : Symbols.cast xs rfl = xs := by
   rcases xs with ⟨xs, rfl⟩
   rfl
 
@@ -111,7 +109,7 @@ theorem Symbols.take_get (xs: Symbols σ (n + m)):
   simp only [Fin.cast_mk, List.get_eq_getElem, List.getElem_take]
 
 theorem Symbols.cast_nil:
-  ⟨[], h1⟩ = Symbols.cast h2 ⟨[], h3⟩ := by
+  ⟨[], h1⟩ = Symbols.cast ⟨[], h3⟩ h2 := by
   subst h3 h1
   simp only [List.length_nil]
   rfl
@@ -122,7 +120,7 @@ theorem Symbols.cons_is_list_cons (x: σ) (xs: List.Vector σ n) (hxs: (x :: xs.
   rfl
 
 theorem Symbols.cast_list {n m: Nat} {σ: Type} (xs: List σ) (h1: xs.length = n) (h2: m = n) (h3: xs.length = m):
-  ⟨xs, h1⟩ = Symbols.cast h2 ⟨xs, h3⟩ := by
+  ⟨xs, h1⟩ = Symbols.cast ⟨xs, h3⟩ h2 := by
   apply List.Vector.eq
   simp
   aesop
@@ -136,12 +134,6 @@ theorem Symbols.take_succ (xs: Symbols α n):
   (Symbols.cast
     (n := ((min i n) + 1))
     (m := (min (i + 1) (n + 1)))
-    (by
-      rw [Nat.min_def]
-      split_ifs
-      omega
-      omega
-    )
     (
       (
         Symbols.cons x (
@@ -150,32 +142,38 @@ theorem Symbols.take_succ (xs: Symbols α n):
       )
       : Symbols α ((min i n) + 1)
     )
+    (by
+      rw [Nat.min_def]
+      split_ifs
+      omega
+      omega
+    )
   )
   := by
   unfold Symbols at *
   apply List.Vector.eq
   rw [<- List.Vector.toList_cast_is_toList]
-  rw [<- List.Vector.toList_take]
-  rw [<- List.Vector.toList_cons]
+  rw [<- Vec.toList_take]
+  rw [<- Vec.toList_cons]
   simp only [List.Vector.cons_val, List.take_succ_cons, List.cons.injEq, true_and]
-  rw [List.Vector.toList_take]
+  rw [Vec.toList_take]
   simp [List.Vector.toList]
 
 theorem Symbols.cast_take (xs: Symbols σ n):
-  Symbols.take n xs = Symbols.cast (n := n) (m := min n n) (by omega) xs := by
+  Symbols.take n xs = Symbols.cast (n := n) (m := min n n) xs (by omega) := by
   unfold Symbols.take
   apply List.Vector.eq
   generalize_proofs h
   rw [<- List.Vector.toList_cast_is_toList]
-  rw [<- List.Vector.toList_take]
+  rw [<- Vec.toList_take]
   rcases xs with ⟨xs, hxs⟩
   simp only [List.Vector.toList_mk, List.take_eq_self_iff]
   omega
 
 theorem Symbols.cast_append_take (xs: Symbols σ n) (ys: Symbols σ m):
-  (xs ++ ys).take n = Symbols.cast (n := n) (m := min n (n + m)) ((by
+  (xs ++ ys).take n = Symbols.cast (n := n) (m := min n (n + m)) xs ((by
     omega
-  ): n = min n (n + m)) xs := by
+  ): n = min n (n + m)) := by
   unfold Symbols at *
   apply List.Vector.eq
   rw [<- List.Vector.toList_cast_is_toList]
@@ -184,8 +182,8 @@ theorem Symbols.cast_append_take (xs: Symbols σ n) (ys: Symbols σ m):
   subst hxs
   simp_all only [List.take_left']
 
-theorem Symbols.push_get {μ: Nat} {α: Type} (xs: Symbols α μ) (x: α):
-  Symbols.get (Symbols.snoc xs x) (Fin.mk μ (by omega)) = x := by
+theorem Symbols.push_get {n: Nat} {α: Type} (xs: Symbols α n) (x: α):
+  Symbols.get (Symbols.snoc xs x) (Fin.mk n (by omega)) = x := by
   unfold Symbols at *
   unfold Symbols.get
   unfold Symbols.snoc
@@ -198,7 +196,7 @@ theorem Symbols.push_get {μ: Nat} {α: Type} (xs: Symbols α μ) (x: α):
   simp only [Fin.cast_mk, List.get_eq_getElem, le_refl, List.getElem_append_right, tsub_self,
     List.getElem_cons_zero]
 
-def replace (r: RegexID μ) (xs: Symbols σ ν) (h: μ <= ν): Regex σ :=
+def replace (r: RegexID n) (xs: Symbols σ l) (h: n <= l): Regex σ :=
   match r with
   | Regex.emptyset => Regex.emptyset
   | Regex.emptystr => Regex.emptystr
@@ -214,14 +212,14 @@ def replace (r: RegexID μ) (xs: Symbols σ ν) (h: μ <= ν): Regex σ :=
   | Regex.star r1 =>
     Regex.star (replace r1 xs h)
 
-theorem replace_cast_both (r: RegexID μ) (xs: Symbols σ μ) (h: μ = ν):
-  replace r xs (by omega) = replace (RegexID.cast h r) (Symbols.cast h xs) (by omega) := by
+theorem replace_cast_both (r: RegexID n) (xs: Symbols σ n) (h: n = l):
+  replace r xs (by omega) = replace (RegexID.cast r h) (Symbols.cast xs h) (by omega) := by
   subst h
   simp only [Symbols.cast_rfl]
   rfl
 
-theorem replace_cast_symbols (r: RegexID μ) (xs: Symbols σ μ) (h: μ = ν):
-  replace r xs (by omega) = replace r (Symbols.cast h xs) (by omega) := by
+theorem replace_cast_symbols (r: RegexID n) (xs: Symbols σ n) (h: n = l):
+  replace r xs (by omega) = replace r (Symbols.cast xs h) (by omega) := by
   subst h
   simp only [Symbols.cast_rfl]
 
@@ -248,8 +246,8 @@ theorem replace_nil_is_map_id (r: Regex (Fin 0)):
     simp [replace, Regex.map]
     rw [ih1]
 
-theorem replace_take (r: RegexID μ) (xs: Symbols σ (μ + n)):
-  replace r (Symbols.take μ xs) (by omega) = replace r xs (by omega):= by
+theorem replace_take (r: RegexID n) (xs: Symbols σ (n + l)):
+  replace r (Symbols.take n xs) (by omega) = replace r xs (by omega):= by
   induction r with
   | emptyset =>
     simp [replace]
@@ -279,8 +277,8 @@ theorem replace_take (r: RegexID μ) (xs: Symbols σ (μ + n)):
     generalize_proofs h1 at *
     rw [<- ih1]
 
-theorem replace_regexid_add (r: RegexID μ) (xs: List.Vector σ (μ + n)):
-  replace r xs (by omega) = replace (RegexID.add n r) xs (by omega):= by
+theorem replace_regexid_add (r: RegexID n) (xs: List.Vector σ (n + l)):
+  replace r xs (by omega) = replace (RegexID.add l r) xs (by omega):= by
   generalize_proofs h1 h2
   rcases xs with ⟨xs, hxs⟩
   induction r with
@@ -309,11 +307,11 @@ theorem replace_regexid_add (r: RegexID μ) (xs: List.Vector σ (μ + n)):
     rw [ih1]
     rfl
 
-def extract (r: Regex σ) (res: Symbols σ μ): RegexID (μ + num r) × Symbols σ (μ + num r) :=
+def extract (r: Regex σ) (res: Symbols σ n): RegexID (n + num r) × Symbols σ (n + num r) :=
   match r with
   | Regex.emptyset => (Regex.emptyset, res)
   | Regex.emptystr => (Regex.emptystr, res)
-  | Regex.symbol s => (Regex.symbol (Fin.mk μ (by
+  | Regex.symbol s => (Regex.symbol (Fin.mk n (by
       simp only [num]
       omega
     )), Symbols.snoc res s)
@@ -329,9 +327,9 @@ def extract (r: Regex σ) (res: Symbols σ μ): RegexID (μ + num r) × Symbols 
     let (er1, res1) := extract r1 res
     (Regex.star er1, res1)
 
-theorem extract_append_toList (res: Symbols σ μ) (r: Regex σ):
+theorem extract_append_toList (res: Symbols σ n) (r: Regex σ):
   List.Vector.toList (extract r res).2 = List.Vector.toList (res ++ (extract r Symbols.nil).2) := by
-  induction r generalizing res μ  with
+  induction r generalizing res n  with
   | emptyset =>
     simp only [num, Nat.add_zero, extract, List.Vector.append_nil]
   | emptystr =>
@@ -375,23 +373,23 @@ theorem extract_append_toList (res: Symbols σ μ) (r: Regex σ):
     simp only [extract]
     rw [ih1]
 
-theorem extract_append (res: Symbols σ μ) (r: Regex σ):
-  (extract r res).2 = Symbols.cast (by omega) (res ++ (extract r Symbols.nil).2) := by
+theorem extract_append (res: Symbols σ l) (r: Regex σ):
+  (extract r res).2 = Symbols.cast (res ++ (extract r Symbols.nil).2) (by omega) := by
   apply List.Vector.eq
   rw [extract_append_toList]
   rw [<- List.Vector.toList_cast_is_toList]
 
-theorem extract_take_toList (res: Symbols σ μ):
+theorem extract_take_toList (res: Symbols σ l):
   (List.Vector.toList
     (List.Vector.take
-      (μ + num r1)
+      (l + num r1)
       (extract r2
       (extract r1 res).2).2
     )
   )
   =
   (List.Vector.toList (extract r1 res).2) := by
-  rw [<- List.Vector.toList_take]
+  rw [<- Vec.toList_take]
   rw [<- List.Vector.toList]
   rw [extract_append_toList]
   rw [List.Vector.toList_append]
@@ -401,72 +399,41 @@ theorem extract_take_toList (res: Symbols σ μ):
   simp only
   simp_all only [List.take_left']
 
-theorem extract_take (res: Symbols σ μ):
+theorem extract_take (res: Symbols σ l):
   (List.Vector.take
-    (μ + num r1)
+    (l + num r1)
     (extract r2
       (extract r1 res).2).2
   )
   =
-    Symbols.cast (by omega)
-    (extract r1 res).2 := by
+    Symbols.cast
+    (extract r1 res).2
+    (by omega) := by
   apply List.Vector.eq
   rw [extract_take_toList]
   rw [<- List.Vector.toList_cast_is_toList]
 
-def replaceFrom (r: RegexID μ) (xs: Symbols σ μ): Regex σ :=
-  match r with
-  | Regex.emptyset => Regex.emptyset
-  | Regex.emptystr => Regex.emptystr
-  | Regex.symbol s => Regex.symbol (Symbols.get xs s)
-  | Regex.or r1 r2 =>
-    Regex.or (replaceFrom r1 xs) (replaceFrom r2 xs)
-  | Regex.concat r1 r2 =>
-    Regex.concat (replaceFrom r1 xs) (replaceFrom r2 xs)
-  | Regex.star r1 =>
-    Regex.star (replaceFrom r1 xs)
+def replaceFrom (r: RegexID n) (xs: Symbols σ n): Regex σ :=
+  replace r xs (le_refl n)
 
-theorem replaceFrom_is_replace (r: RegexID μ) (xs: Symbols σ μ):
-  replaceFrom r xs = replace r xs (le_refl μ) := by
-  induction r with
-  | emptyset =>
-    simp [replaceFrom, replace]
-  | emptystr =>
-    simp [replaceFrom, replace]
-  | symbol s =>
-    simp [replaceFrom, replace]
-  | or r1 r2 ih1 ih2 =>
-    simp [replaceFrom, replace]
-    rw [ih1]
-    rw [ih2]
-    apply And.intro rfl rfl
-  | concat r1 r2 ih1 ih2 =>
-    simp [replaceFrom, replace]
-    rw [ih1]
-    rw [ih2]
-    apply And.intro rfl rfl
-  | star r1 ih1 =>
-    simp [replaceFrom, replace]
-    rw [ih1]
-
-theorem extract_replaceFrom_is_id (r: Regex σ) (res: Symbols σ μ):
+theorem extract_replaceFrom_is_id (r: Regex σ) (res: Symbols σ l):
   r = replaceFrom (extract r res).1 (extract r res).2 := by
-  rw [replaceFrom_is_replace]
+  simp only [replaceFrom]
   generalize_proofs hr
-  revert res μ
+  revert res l
   induction r with
   | emptyset =>
-    intro μ res hr
+    intro n res hr
     simp only [replace, extract]
   | emptystr =>
-    intro μ res hr
+    intro n res hr
     simp only [replace, extract]
   | symbol s =>
-    intro μ res hr
+    intro n res hr
     simp only [replace, extract]
     rw [Symbols.push_get]
   | or r1 r2 ih1 ih2 =>
-    intro μ res hr
+    intro n res hr
     simp only [extract]
     simp only [replace]
     have hh1 :
@@ -497,7 +464,7 @@ theorem extract_replaceFrom_is_id (r: Regex σ) (res: Symbols σ μ):
     rw [<- replace_cast_both]
     rw [<- ih2 ((extract r1 res).2)]
   | concat r1 r2 ih1 ih2 =>
-    intro μ res hr
+    intro n res hr
     simp only [extract]
     simp only [replace]
     have hh1 :
@@ -530,10 +497,98 @@ theorem extract_replaceFrom_is_id (r: Regex σ) (res: Symbols σ μ):
   | star r1 ih1 =>
     simp only [extract]
     simp only [replace]
-    intro μ res hr
+    intro n res hr
     rw [<- ih1 res]
 
-theorem extract_replace_is_id (r: Regex σ) (res: Symbols σ μ):
+theorem extract_replace_is_id (r: Regex σ) (res: Symbols σ l):
   r = replace (extract r res).1 (extract r res).2 (by omega):= by
-  rw [<- replaceFrom_is_replace]
+  rw [<- replaceFrom]
   rw [<- extract_replaceFrom_is_id]
+
+def extractFrom (r: Regex σ): RegexID (num r) × Symbols σ (num r) :=
+  match extract r List.Vector.nil with
+  | (r', xs) => (RegexID.cast r' (by omega), Symbols.cast xs (by omega))
+
+theorem extractFrom_replaceFrom_is_id (r: Regex σ):
+  r = replaceFrom (extractFrom r).1 (extractFrom r).2 := by
+  simp only [extractFrom]
+  simp only [replaceFrom]
+  rw [<- replace_cast_both]
+  rw [<- extract_replace_is_id r List.Vector.nil]
+
+theorem nums_cons_is_add:
+  nums (⟨x::xs, h⟩)
+  = num x + nums ⟨xs, congrArg Nat.pred h⟩
+  := by
+  simp [nums]
+  ac_rfl
+
+theorem RegexID.cons_cast:
+  List.Vector (RegexID (nres + nums (⟨x::xs, h⟩))) n
+  = List.Vector (RegexID (nres + num x + nums ⟨xs, congrArg Nat.pred h⟩)) n := by
+  simp [nums]
+  ac_rfl
+
+def extracts (xs: List.Vector (Regex σ) nregex) (res: Symbols σ nres):
+  (List.Vector (RegexID (nres + nums xs)) nregex) × (Symbols σ (nres + nums xs)) :=
+  match xs with
+  | ⟨[], h⟩ =>
+    (
+      ⟨[], by assumption ⟩,
+      ⟨res.val, by simp only [List.Vector.length_val, nums, add_zero]⟩
+    )
+  | ⟨x::xs, h⟩ =>
+    let xs': List.Vector (Regex σ) nregex.pred := ⟨xs, congrArg Nat.pred h⟩
+    let (regex, symbols) := Symbol.extract x res
+    let regex' := RegexID.add (nums ⟨xs, congrArg Nat.pred h⟩) regex
+    let regex'': RegexID (nres + nums (⟨x::xs, h⟩)) :=
+      RegexID.cast
+      regex'
+      (by
+        simp
+        rw [nums_cons_is_add]
+        ac_rfl
+      )
+    let (regexes, symbols') := extracts xs' symbols
+    let regexes': List.Vector (RegexID (nres + nums (⟨x::xs, h⟩))) nregex.pred
+      := by
+        rw [RegexID.cons_cast]
+        exact regexes
+    let regexes'' : List.Vector (RegexID (nres + nums (⟨x::xs, h⟩))) nregex :=
+      (Symbols.cast
+        ((List.Vector.cons
+          regex''
+          regexes'
+        ): List.Vector (RegexID (nres + nums (⟨x::xs, h⟩))) nregex.pred.succ)
+        (by
+          rw [<- h]
+          simp only [List.length_cons, Nat.pred_eq_sub_one, add_tsub_cancel_right, Nat.succ_eq_add_one]
+        )
+      )
+    let symbols': Symbols σ (nres + nums (⟨x::xs, h⟩)) :=
+      Symbols.cast
+      symbols'
+      (by
+        simp [nums]
+        ac_rfl
+      )
+    (
+      regexes'',
+      symbols'
+    )
+
+def extractsSymbols (xs: List.Vector (Regex σ) l1) (res: Symbols σ l2):
+  Symbols σ (l2 + Symbol.nums xs) :=
+  match xs with
+  | ⟨[], h⟩ => ⟨res.val, by simp only [List.Vector.length_val, Symbol.nums, add_zero]⟩
+  | ⟨x::xs, h⟩ =>
+      (Symbol.Symbols.cast
+        (extractsSymbols ⟨xs, congrArg Nat.pred h⟩ (Symbol.extract x res).2)
+        (by simp only [Symbol.nums]; ac_rfl)
+      )
+
+def extracts_list (xs: List (Regex σ)) (res: List σ):
+  (List (RegexID (res.length + nums_list xs))) × (List σ) :=
+  let (r1, r2) := extracts (Vec.fromList xs) (Vec.fromList res)
+  let r2List: List σ := List.Vector.toList r2
+  (r1.toList, r2List)
