Validator/Memoize/MemEnter.lean
@@ -5,32 +5,62 @@ import Validator.Std.Debug
 import Validator.Expr.Grammar
 import Validator.Expr.IfExpr
 import Validator.Expr.Regex
+import Validator.Expr.Symbol
 
 import Validator.Derive.Enter
 
-abbrev MemEnter.EnterMap (μ: Nat) α [DecidableEq α] [Hashable α] := Std.ExtHashMap (Rules μ α Pred) (IfExprs μ α)
-def MemEnter.EnterMap.mk [DecidableEq α] [Hashable α] : EnterMap μ α := Std.ExtHashMap.emptyWithCapacity
+abbrev MemEnter.EnterMap (n: Nat) α [DecidableEq α] [Hashable α] :=
+  Std.ExtDHashMap
+    Nat
+    (fun l =>
+      Std.ExtDHashMap
+        (Rules n (Pred α) l)
+        (fun xs =>
+          (IfExprs n α (Symbol.nums xs))
+        )
+    )
 
-class MemEnter (m: Type -> Type u) (μ: outParam Nat) (α: outParam Type) [DecidableEq α] [Hashable α] where
-  getEnter : m (MemEnter.EnterMap μ α)
-  setEnter : (MemEnter.EnterMap μ α) → m Unit
+def MemEnter.EnterMap.mk [DecidableEq α] [Hashable α] : EnterMap n α := Std.ExtDHashMap.emptyWithCapacity
+
+class MemEnter (m: Type -> Type u) (n: outParam Nat) (α: outParam Type) [DecidableEq α] [Hashable α] where
+  getEnter : m (MemEnter.EnterMap n α)
+  setEnter : (MemEnter.EnterMap n α) → m Unit
 
 namespace MemEnter
 
+def get? [DecidableEq α] [Hashable α] (m: MemEnter.EnterMap n α) (xs: Rules n (Pred α) l): Option (IfExprs n α (Symbol.nums xs)) :=
+  match m.get? l with
+  | Option.none => Option.none
+  | Option.some mxs =>
+    match mxs.get? xs with
+    | Option.none => Option.none
+    | Option.some ifs => Option.some ifs
+
+def insert [DecidableEq α] [Hashable α]
+  (m: MemEnter.EnterMap n α)
+  (key: Rules n (Pred α) l)
+  (value: IfExprs n α (Symbol.nums key))
+  : MemEnter.EnterMap n α :=
+  match m.get? l with
+  | Option.none =>
+    m.insert l (Std.ExtDHashMap.emptyWithCapacity.insert key value)
+  | Option.some mxs =>
+    m.insert l (mxs.insert key value)
+
 def deriveEnter
   [DecidableEq α] [Hashable α]
-  [Monad m] [Debug m] [MemEnter m μ α]
-  (xs: Rules μ α Pred): m (IfExprs μ α) := do
+  [Monad m] [Debug m] [MemEnter m n α]
+  {l: Nat} (xs: Rules n (Pred α) l): m (IfExprs n α (Symbol.nums xs)) := do
   let memoized <- MemEnter.getEnter
-  match memoized.get? xs with
+  match get? memoized xs with
   | Option.none =>
     Debug.debug "cache miss"
     let newvalue := Enter.deriveEnter xs
-    MemEnter.setEnter (memoized.insert xs newvalue)
+    MemEnter.setEnter (insert memoized xs newvalue)
     return newvalue
   | Option.some value =>
     Debug.debug "cache hit"
     return value
 
-instance [DecidableEq α] [Hashable α] [Monad m] [Debug m] [MemEnter m μ α] : Enter.DeriveEnter m μ α where
-  deriveEnter (xs: Rules μ α Pred): m (IfExprs μ α) := deriveEnter xs
+instance [DecidableEq α] [Hashable α] [Monad m] [Debug m] [MemEnter m n α] : Enter.DeriveEnter m n α where
+  deriveEnter {l: Nat} (xs: Rules n (Pred α) l): m (IfExprs n α (Symbol.nums xs)) := deriveEnter xs
