Validator/Memoize/MemLeave.lean
@@ -5,32 +5,66 @@ import Validator.Std.Debug
 import Validator.Expr.Grammar
 import Validator.Expr.IfExpr
 import Validator.Expr.Regex
+import Validator.Expr.Symbol
 
 import Validator.Derive.Leave
 
-abbrev MemLeave.LeaveMap μ α [DecidableEq α] [Hashable α] := Std.ExtHashMap (Rules μ α Pred × List Bool) (Rules μ α Pred)
-def MemLeave.LeaveMap.mk [DecidableEq α] [Hashable α]: LeaveMap μ α := Std.ExtHashMap.emptyWithCapacity
+def hashRulesAndNulls {n: Nat} {Φ: Type} {l: Nat} [Hashable Φ] (x: (xs: Rules n Φ l) × (List.Vector Bool (Symbol.nums xs))): UInt64 :=
+  mixHash (hash x.1) (hash x.2)
 
-class MemLeave (m: Type -> Type u) (μ: outParam Nat) (α: outParam Type) [DecidableEq α] [Hashable α] where
-  getLeave : m (MemLeave.LeaveMap μ α)
-  setLeave : MemLeave.LeaveMap μ α → m Unit
+instance (n: Nat) (Φ: Type) (l: Nat) [Hashable Φ] : Hashable ((xs: Rules n Φ l) × (List.Vector Bool (Symbol.nums xs))) where
+  hash := hashRulesAndNulls
+
+abbrev MemLeave.LeaveMap n α [DecidableEq α] [Hashable α] :=
+  Std.ExtDHashMap
+    Nat
+    (fun l =>
+      Std.ExtHashMap
+        ((xs: Rules n (Pred α) l) × (List.Vector Bool (Symbol.nums xs)))
+        (Rules n (Pred α) l)
+    )
+
+def MemLeave.LeaveMap.mk [DecidableEq α] [Hashable α]: LeaveMap n α := Std.ExtDHashMap.emptyWithCapacity
+
+class MemLeave (m: Type -> Type u) (n: outParam Nat) (α: outParam Type) [DecidableEq α] [Hashable α] where
+  getLeave : m (MemLeave.LeaveMap n α)
+  setLeave : MemLeave.LeaveMap n α → m Unit
 
 namespace MemLeave
 
+def get? [DecidableEq α] [Hashable α]
+  (m: MemLeave.LeaveMap n α)
+  (key: (xs: Rules n (Pred α) l) × (List.Vector Bool (Symbol.nums xs)))
+  : Option (Rules n (Pred α) l) :=
+  match m.get? l with
+  | Option.none => Option.none
+  | Option.some mkey => mkey.get? key
+
+def insert [DecidableEq α] [Hashable α]
+  (m: MemLeave.LeaveMap n α)
+  (key: (xs: Rules n (Pred α) l) × (List.Vector Bool (Symbol.nums xs)))
+  (value: Rules n (Pred α) l) :=
+  match m.get? l with
+  | Option.none =>
+    m.insert l (Std.ExtHashMap.emptyWithCapacity.insert key value)
+  | Option.some mxs =>
+    m.insert l (mxs.insert key value)
+
 def deriveLeaveM
   [DecidableEq α] [Hashable α]
-  [Monad m] [Debug m] [MonadExcept String m] [MemLeave m μ α]
-  (xs: Rules μ α Pred) (ns: List Bool): m (Rules μ α Pred) := do
+  [Monad m] [Debug m] [MonadExcept String m] [MemLeave m n α]
+  (xs: Rules n (Pred α) l) (ns: List.Vector Bool (Symbol.nums xs)): m (Rules n (Pred α) l) := do
   let memoized <- MemLeave.getLeave
-  match memoized.get? (xs, ns) with
+  let key: ((xs: Rules n (Pred α) l) × (List.Vector Bool (Symbol.nums xs))) := Sigma.mk xs ns
+  match get? memoized key with
   | Option.none =>
     Debug.debug "cache miss"
-    let newvalue <- Leave.deriveLeaveM xs ns
-    MemLeave.setLeave (memoized.insert (xs, ns) newvalue)
+    let newvalue := Leave.deriveLeaves xs ns
+    MemLeave.setLeave (insert memoized key newvalue)
     return newvalue
   | Option.some value =>
     Debug.debug "cache hit"
     return value
 
-instance [DecidableEq α] [Hashable α] [Monad m] [Debug m] [MonadExcept String m] [MemLeave m μ α] : Leave.DeriveLeaveM m μ α where
-  deriveLeaveM (xs: Rules μ α Pred) (ns: List Bool): m (Rules μ α Pred) := deriveLeaveM xs ns
+instance [DecidableEq α] [Hashable α] [Monad m] [Debug m] [MonadExcept String m] [MemLeave m n α] : Leave.DeriveLeaveM m n α where
+  deriveLeaveM {l: Nat} (xs: Rules n (Pred α) l) (ns: List.Vector Bool (Symbol.nums xs)): m (Rules n (Pred α) l) := deriveLeaveM xs ns
