Validator/Validator/Validate.lean
@@ -21,19 +21,19 @@ import Validator.Validator.Inst.TreeParserMemM
 
 namespace Validate
 
-def deriveEnter [DecidableEq α] [ValidateM m μ α] (g: Grammar μ α Pred) (xs: Rules μ α Pred): m (Rules μ α Pred) := do
+def deriveEnter [DecidableEq α] [ValidateM m n α] (g: Grammar n (Pred α)) (xs: Rules n (Pred α) l): m (Rules n (Pred α) (Symbol.nums xs)) := do
   let token <- Parser.token
   let enters <- Enter.DeriveEnter.deriveEnter xs
   return IfExpr.evals g enters token
 
-def deriveLeaveM [ValidateM m μ α] (xs: Rules μ α Pred) (cs: Rules μ α Pred): m (Rules μ α Pred) :=
-  Leave.DeriveLeaveM.deriveLeaveM xs (List.map Rule.nullable cs)
+def deriveLeaveM [ValidateM m n α] (xs: Rules n (Pred α) l) (cs: Rules n (Pred α) (Symbol.nums xs)): m (Rules n (Pred α) l) :=
+  Leave.DeriveLeaveM.deriveLeaveM xs (List.Vector.map Rule.nullable cs)
 
-def deriveValue [DecidableEq α] [ValidateM m μ α] (g: Grammar μ α Pred) (xs: Rules μ α Pred): m (Rules μ α Pred) := do
+def deriveValue [DecidableEq α] [ValidateM m n α] (g: Grammar n (Pred α)) (xs: Rules n (Pred α) l): m (Rules n (Pred α) l) := do
   deriveLeaveM xs (<- deriveEnter g xs)
 
-partial def derive [DecidableEq α] [ValidateM m μ α] (g: Grammar μ α Pred) (xs: Rules μ α Pred): m (Rules μ α Pred) := do
-  if List.all xs Regex.unescapable then
+partial def derive [DecidableEq α] [ValidateM m n α] (g: Grammar n (Pred α)) (xs: Rules n (Pred α) l): m (Rules n (Pred α) l) := do
+  if List.all xs.toList Regex.unescapable then
     Parser.skip; return xs
   match <- Parser.next with
   | Hint.field =>
@@ -42,7 +42,7 @@ partial def derive [DecidableEq α] [ValidateM m μ α] (g: Grammar μ α Pred) 
       match <- Parser.next with
       | Hint.value => deriveValue g childxs -- derive child value
       | Hint.enter =>
-        let (cchildxs, indices) <- Compress.compressM childxs -- NEW: compress
+        let ⟨_, cchildxs, indices⟩ <- Compress.compressM childxs -- NEW: compress
         let cdchildxs <- derive g cchildxs -- derive children, until return from a Hint.leave
         Compress.expandM indices cdchildxs -- NEW: expand
       | hint => throw s!"unexpected {hint}"
@@ -50,21 +50,19 @@ partial def derive [DecidableEq α] [ValidateM m μ α] (g: Grammar μ α Pred) 
     derive g xsLeave -- deriv next
   | Hint.value => deriveValue g xs >>= derive g -- derive value and then derive next
   | Hint.enter =>
-    let (cchildxs, indices) <- Compress.compressM xs -- NEW: compress
+    let ⟨_, cchildxs, indices⟩ <- Compress.compressM xs -- NEW: compress
     let cdchildxs <- derive g cchildxs -- derive children, until return from a Hint.leave
     let dchildxs <- Compress.expandM indices cdchildxs -- NEW: expand
     derive g dchildxs -- derive next
   | Hint.leave => return xs -- never happens at the top
   | Hint.eof => return xs -- only happens at the top
 
-def validate {m} {μ: Nat} {α: Type} [DecidableEq α] [ValidateM m μ α] (g: Grammar μ α Pred) (x: Rule μ α Pred): m Bool := do
-  let dxs <- derive g [x]
-  match dxs with
-  | [dx] => return Rule.nullable dx
-  | _ => throw "expected one expression"
+def validate {m} {n: Nat} {α: Type} [DecidableEq α] [ValidateM m n α] (g: Grammar n (Pred α)) (x: Rule n (Pred α)): m Bool := do
+  let dxs <- derive g (List.Vector.cons x List.Vector.nil)
+  return Rule.nullable dxs.head
 
-def run {μ: Nat} {α: Type} [DecidableEq α] [Hashable α] (g: Grammar μ α Pred) (t: Hedge.Node α): Except String Bool :=
-  TreeParserMemM.run' (μ := μ) (validate g g.start) t
+def run {α: Type} [DecidableEq α] [Hashable α] (g: Grammar n (Pred α)) (t: Hedge.Node α): Except String Bool :=
+  TreeParserMemM.run' (n := n) (validate g g.start) t
 
 -- Tests
 
@@ -76,7 +74,7 @@ open TokenTree (node)
   Except.ok false
 
 #guard run
-  (Grammar.mk (μ := 1)
+  (Grammar.mk (n := 1)
     (Regex.symbol (Pred.eq (Token.string "a"), 0))
     #v[Regex.emptystr]
   )
@@ -84,7 +82,7 @@ open TokenTree (node)
   Except.ok true
 
 #guard run
-  (Grammar.mk (μ := 1)
+  (Grammar.mk (n := 1)
     (Regex.symbol (Pred.eq (Token.string "a"), 0))
     #v[Regex.emptystr]
   )
@@ -92,7 +90,7 @@ open TokenTree (node)
   Except.ok false
 
 #guard run
-  (Grammar.mk (μ := 2)
+  (Grammar.mk (n := 2)
     (Regex.symbol (Pred.eq (Token.string "a"), 0))
     #v[
       (Regex.symbol (Pred.eq (Token.string "b"), 1))
@@ -103,7 +101,7 @@ open TokenTree (node)
   = Except.ok true
 
 #guard run
-  (Grammar.mk (μ := 2)
+  (Grammar.mk (n := 2)
     (Regex.symbol (Pred.eq (Token.string "a"), 0))
     #v[
       (Regex.concat
@@ -117,7 +115,7 @@ open TokenTree (node)
   Except.ok true
 
 #guard run
-  (Grammar.mk (μ := 3)
+  (Grammar.mk (n := 3)
     (Regex.symbol (Pred.eq (Token.string "a"), 0))
     #v[
       (Regex.concat
@@ -133,7 +131,7 @@ open TokenTree (node)
 
 -- try to engage skip using emptyset, since it is unescapable
 #guard run
-  (Grammar.mk (μ := 1)
+  (Grammar.mk (n := 1)
     (Regex.symbol (Pred.eq (Token.string "a"), 0))
     #v[Regex.emptyset]
   )
@@ -141,7 +139,7 @@ open TokenTree (node)
   = Except.ok false
 
 #guard run
-  (Grammar.mk (μ := 4)
+  (Grammar.mk (n := 4)
     (Regex.symbol (Pred.eq (Token.string "a"), 0))
     #v[
       (Regex.concat
@@ -157,7 +155,7 @@ open TokenTree (node)
   = Except.ok false
 
 #guard run
-  (Grammar.mk (μ := 2)
+  (Grammar.mk (n := 2)
     (Regex.symbol (Pred.eq (Token.string "a"), 0))
     #v[
       (Regex.concat
@@ -171,7 +169,7 @@ open TokenTree (node)
   Except.ok false
 
 #guard run
-  (Grammar.mk (μ := 3)
+  (Grammar.mk (n := 3)
     (Regex.symbol (Pred.eq (Token.string "a"), 0))
     #v[
       (Regex.concat
@@ -186,7 +184,7 @@ open TokenTree (node)
   = Except.ok false
 
 #guard run
-  (Grammar.mk (μ := 4)
+  (Grammar.mk (n := 4)
     (Regex.symbol (Pred.eq (Token.string "a"), 0))
     #v[
       (Regex.concat
