Validator/Learning/Memoize.lean
@@ -8,11 +8,11 @@ import Validator.Learning.Parser
 
 namespace Memoize
 
-def validate {m} [DecidableEq α] [ValidateM m μ α] (g: Grammar μ α Pred) (x: Rule μ α Pred): m Bool :=
+def validate {m} [DecidableEq α] [ValidateM m n α] (g: Grammar n (Pred α)) (x: Rule n (Pred α)): m Bool :=
   Parser.validate g x
 
-def run [DecidableEq α] [Hashable α] (g: Grammar μ α Pred) (t: Hedge.Node α): Except String Bool :=
-  TreeParserMemM.run' (μ := μ) (validate g g.start) t
+def run [DecidableEq α] [Hashable α] (g: Grammar n (Pred α)) (t: Hedge.Node α): Except String Bool :=
+  TreeParserMemM.run' (n := n) (validate g g.start) t
 
 -- Tests
 
@@ -24,7 +24,7 @@ open TokenTree (node)
   Except.ok false
 
 #guard run
-  (Grammar.mk (μ := 1)
+  (Grammar.mk (n := 1)
     (Regex.symbol (Pred.eq (Token.string "a"), 0))
     #v[Regex.emptystr]
   )
@@ -32,7 +32,7 @@ open TokenTree (node)
   Except.ok true
 
 #guard run
-  (Grammar.mk (μ := 1)
+  (Grammar.mk (n := 1)
     (Regex.symbol (Pred.eq (Token.string "a"), 0))
     #v[Regex.emptystr]
   )
@@ -40,7 +40,7 @@ open TokenTree (node)
   Except.ok false
 
 #guard run
-  (Grammar.mk (μ := 2)
+  (Grammar.mk (n := 2)
     (Regex.symbol (Pred.eq (Token.string "a"), 0))
     #v[
       (Regex.symbol (Pred.eq (Token.string "b"), 1))
@@ -51,7 +51,7 @@ open TokenTree (node)
   = Except.ok true
 
 #guard run
-  (Grammar.mk (μ := 2)
+  (Grammar.mk (n := 2)
     (Regex.symbol (Pred.eq (Token.string "a"), 0))
     #v[
       (Regex.concat
@@ -65,7 +65,7 @@ open TokenTree (node)
   Except.ok true
 
 #guard run
-  (Grammar.mk (μ := 3)
+  (Grammar.mk (n := 3)
     (Regex.symbol (Pred.eq (Token.string "a"), 0))
     #v[
       (Regex.concat
@@ -81,7 +81,7 @@ open TokenTree (node)
 
 -- try to engage skip using emptyset, since it is unescapable
 #guard run
-  (Grammar.mk (μ := 1)
+  (Grammar.mk (n := 1)
     (Regex.symbol (Pred.eq (Token.string "a"), 0))
     #v[Regex.emptyset]
   )
@@ -89,7 +89,7 @@ open TokenTree (node)
   = Except.ok false
 
 #guard run
-  (Grammar.mk (μ := 4)
+  (Grammar.mk (n := 4)
     (Regex.symbol (Pred.eq (Token.string "a"), 0))
     #v[
       (Regex.concat
@@ -105,7 +105,7 @@ open TokenTree (node)
   = Except.ok false
 
 #guard run
-  (Grammar.mk (μ := 2)
+  (Grammar.mk (n := 2)
     (Regex.symbol (Pred.eq (Token.string "a"), 0))
     #v[
       (Regex.concat
@@ -119,7 +119,7 @@ open TokenTree (node)
   Except.ok false
 
 #guard run
-  (Grammar.mk (μ := 3)
+  (Grammar.mk (n := 3)
     (Regex.symbol (Pred.eq (Token.string "a"), 0))
     #v[
       (Regex.concat
@@ -134,7 +134,7 @@ open TokenTree (node)
   = Except.ok false
 
 #guard run
-  (Grammar.mk (μ := 4)
+  (Grammar.mk (n := 4)
     (Regex.symbol (Pred.eq (Token.string "a"), 0))
     #v[
       (Regex.concat
