Validator/Std/Vec.lean
@@ -1,0 +1,18 @@
+import Mathlib.Data.Vector.Basic
+import Mathlib.Data.Vector.Snoc
+import Mathlib.Data.Vector.MapLemmas
+
+namespace Vec
+
+def fromList (xs: List α): List.Vector α (xs.length) :=
+  Subtype.mk xs rfl
+
+theorem toList_take:
+  List.take n xs.val = (List.Vector.take n xs).toList := by
+  simp only [_root_.List.Vector.toList_take]
+  rfl
+
+theorem toList_cons:
+  List.cons x xs.val = (List.Vector.cons x xs).toList := by
+  simp only [Nat.succ_eq_add_one, _root_.List.Vector.toList_cons, List.cons.injEq, true_and]
+  rfl
